Bernoulli imperative equivalence

Library/Model/Bernoulli.dfy
@@ -20,7 +20,7 @@ module Bernoulli {
 
   // Equation (4.23)
   function ProbBernoulli(p: Probability): Hurd<bool> {
-    assume {:axiom} false;
+    assume {:axiom} false; // Assume termination
     var f :=
       (b: bool) =>
         if b then
@@ -34,16 +34,59 @@ module Bernoulli {
           else
             Return(true);
     Bind(Deconstruct, f)
-  }  
+  }
+
+  function ProbBernoulliNext(p': Probability, b: bool): (p: Probability)
+    requires (b && p' > 0.5) || (!b && p' <= 0.5)
+  {
+    if (b && p' > 0.5) then 
+      2.0 * p' - 1.0
+    else
+      2.0 * p'
+  }
+
+  function ProbBernoulliCurried(p: Probability, s: RNG): (t: (bool, RNG))
+    ensures t == ProbBernoulli(p)(s)
+  {
+    if Head(s) then
+      if p <= 0.5 then 
+        (false, Tail(s))
+      else
+        assume {:axiom} false; // Assume termination
+        ProbBernoulliCurried(2.0 * p - 1.0, Tail(s))
+    else
+      if p <= 0.5 then
+        assume {:axiom} false; // Assume termination
+        ProbBernoulliCurried(2.0 * p, Tail(s))
+      else
+        (true, Tail(s))
+  }
+
+/*   function ProbBernoulli(p: Probability, s: RNG, ghost w: nat): (bool, RNG)
+    decreases w
+  {
+    assume {:axiom} w != 0; // Assume termination
+
+    if Head(s) then 
+      if p <= 0.5 then 
+        (false, s)
+      else 
+        ProbBernoulli(2.0 * p - 1.0, Tail(s), w - 1)
+    else 
+      if p <= 0.5 then
+        ProbBernoulli(2.0 * p, Tail(s), w - 1)
+      else
+        (true, s)
+  }   */
 
   /*******
    Lemmas  
   *******/
 
-  lemma {:axiom} ProbBernoulliIsIndepFn(p: Probability)
+  lemma {:axiom} ProbBernoulliIsIndepFn(p: Probability, w: nat)
     ensures IsIndepFn(ProbBernoulli(p))
 
-  lemma {:axiom} BernoulliCorrectness(p: Probability)
+  lemma {:axiom} BernoulliCorrectness(p: Probability, w: nat)
     ensures 
       var e := iset s | ProbBernoulli(p)(s).0;
       && e in event_space
