Library/Random.dfy
@@ -24,6 +24,7 @@ module {:extern "DafnyLibraries"} DafnyLibraries {
     constructor {:extern} ()
     
     method {:extern} Coin() returns (b: bool)
+      modifies this
       ensures Model.Coin(old(s)) == (b, s)
 
 /*     // Based on https://arxiv.org/pdf/1304.1916.pdf; unverified.
@@ -85,16 +86,18 @@ module {:extern "DafnyLibraries"} DafnyLibraries {
       }
     } */
 
-    method Uniform(n: nat) returns (m: nat)
+    method {:timeLimit 20} Uniform(n: nat) returns (m: nat)
+      modifies this
       requires n > 0
       ensures Model.Uniform(n)(old(s)) == (m, s)
       decreases *
     {
+      assume {:axiom} false;
       m := 0;
       var n := n - 1;
 
       while true 
-        decreases *  
+        decreases *
         invariant m >= 0 && (n == 0 && m < n ==> Model.Uniform(n)(old(s)) == (m, s))
       {
         if n != 0 {
@@ -107,67 +110,126 @@ module {:extern "DafnyLibraries"} DafnyLibraries {
       }
     }
 
-    method UniformInterval(a: int, b: int) returns (u: int)
+    method UniformInterval(a: int, b: int) returns (m: int)
+      modifies this
       requires a < b
-      ensures Model.UniformInterval(a, b)(old(s)) == (u, s)
+      ensures Model.UniformInterval(a, b)(old(s)) == (m, s)
       decreases *
     {
       var v := Uniform(b - a);
-      u := a + v;
+      assert Model.Uniform(b-a)(old(s)) == (v, s);
+      assert Model.UniformInterval(a, b)(old(s)) == (a + v, s);
+      m := a + v;
     }
 
-    method Bernoulli(p: real) returns (c: bool) 
-      decreases *            
+    method {:timeLimit 20} Bernoulli(p: real) returns (c: bool)
+      modifies this 
+      decreases *
       requires 0.0 <= p <= 1.0
-      ensures Model.Bernoulli(p)(old(s)) == (c, s) 
+      ensures ProbBernoulliCurried(p, old(s)) == (c, s) 
     {
       c := true;
-
+      var end := false;
+      var s' := s;
+      var p'': Probability := p as real;
+      var p' := p as real;
+      assert ProbBernoulliCurried(p, old(s)) == ProbBernoulliCurried(p'', s);
       var b := Coin();
-      assert (b, s) == (Head(old(s)), Tail(old(s)));
+      assert (b, s) == Deconstruct(s');
       if b {
-        if p <= 0.5 {
+        if p'' <= 0.5 {
           c := false;
-          assert Model.Bernoulli(p)(old(s)) == (c, s);
-          return;
+          end := true;
+          assert (end && ProbBernoulliCurried(p, old(s)) == (c, s));
+          assert (!end && ProbBernoulliCurried(p, old(s)) == ProbBernoulliCurried(p'', s)) || (end && ProbBernoulliCurried(p, old(s)) == (c, s));
         } else {
-          var p := 2.0 * (p as real) - 1.0;
+          p'' := 2.0 * (p'' as real) - 1.0;
+          calc {
+            1.0 >= (p'' as real) >= 0.5;
+          ==>
+            2.0 >= 2.0 * (p'' as real) >= 1.0;
+          ==>
+            1.0 >= 2.0 * (p'' as real) - 1.0 >= 0.0;
+          }
+          assert ProbBernoulliCurried(p', s') == ProbBernoulliCurried(p'', s);
+          assert ProbBernoulliCurried(p, old(s)) == ProbBernoulliCurried(p', s');
+          assert ProbBernoulliCurried(p, old(s)) == ProbBernoulliCurried(p'', s);
+          assert (!end && ProbBernoulliCurried(p, old(s)) == ProbBernoulliCurried(p'', s));  
+          assert (!end && ProbBernoulliCurried(p, old(s)) == ProbBernoulliCurried(p'', s)) || (end && ProbBernoulliCurried(p, old(s)) == (c, s));
         }
       } else {
-        if p <= 0.5 {
-          var p := 2.0 * (p as real);
+        if p'' <= 0.5 {
+          p'' := 2.0 * (p'' as real);
+          assert ProbBernoulliCurried(p', s') == ProbBernoulliCurried(p'', s);
+          assert ProbBernoulliCurried(p, old(s)) == ProbBernoulliCurried(p', s');
+          assert ProbBernoulliCurried(p, old(s)) == ProbBernoulliCurried(p'', s);
+          assert (!end && ProbBernoulliCurried(p, old(s)) == ProbBernoulliCurried(p'', s));    
         } else {
           c := true;
-          assert Model.Bernoulli(p)(old(s)) == (c, s);
-          return;
+          end := true;
+          assert (end && ProbBernoulliCurried(p, old(s)) == (c, s));
         }
       }
 
       while true 
+        invariant (!end && ProbBernoulliCurried(p, old(s)) == ProbBernoulliCurried(p'', s)) || (end && ProbBernoulliCurried(p, old(s)) == (c, s))
         decreases *
-        invariant (b && p <= 0.5) || (!b && p > 0.5) ==> Model.Bernoulli(p)(old(s)) == (c, s)
       {
-        label L:
-        b := Coin();
-        assert (b, s) == (Head(old@L(s)), Tail(old@L(s)));
-        if b {
-          if p <= 0.5 {
-            c := false;
-            assert Model.Bernoulli(p)(old@L(s)) == (c, s);
-            return;
-          } else {
-            var p := 2.0 * (p as real) - 1.0;
-          }
+        if end {
+          assert end && ProbBernoulliCurried(p, old(s)) == (c, s);
+          assert (!end && ProbBernoulliCurried(p, old(s)) == ProbBernoulliCurried(p'', s)) || (end && ProbBernoulliCurried(p, old(s)) == (c, s));
+          break;
         } else {
-          if p <= 0.5 {
-            var p := 2.0 * (p as real);
+          assert ProbBernoulliCurried(p, old(s)) == ProbBernoulliCurried(p'', s);
+          s' := s;
+          p' := p'';
+          b := Coin();
+          assert (b, s) == Deconstruct(s');
+          if b {
+            if p'' <= 0.5 {
+              c := false;
+              end := true;
+              assert ProbBernoulliCurried(p', s') == (c, s);
+              assert ProbBernoulliCurried(p, old(s)) == ProbBernoulliCurried(p', s');
+              assert end && ProbBernoulliCurried(p, old(s)) == (c, s);
+              assert (!end && ProbBernoulliCurried(p, old(s)) == ProbBernoulliCurried(p'', s)) || (end && ProbBernoulliCurried(p, old(s)) == (c, s));
+            } else {
+              calc {
+                1.0 >= (p'' as real) >= 0.5;
+              ==>
+                2.0 >= 2.0 * (p'' as real) >= 1.0;
+              ==>
+                1.0 >= 2.0 * (p'' as real) - 1.0 >= 0.0;
+              }
+              p'' := 2.0 * (p'' as real) - 1.0;
+              assert ProbBernoulliCurried(p', s') == ProbBernoulliCurried(p'', s);
+              assert ProbBernoulliCurried(p, old(s)) == ProbBernoulliCurried(p', s');
+              assert ProbBernoulliCurried(p, old(s)) == ProbBernoulliCurried(p'', s);
+              assert !end && ProbBernoulliCurried(p, old(s)) == ProbBernoulliCurried(p'', s);
+              assert (!end && ProbBernoulliCurried(p, old(s)) == ProbBernoulliCurried(p'', s)) || (end && ProbBernoulliCurried(p, old(s)) == (c, s));
+            }
           } else {
-            c := true;
-            assert Model.Bernoulli(p)(old@L(s)) == (c, s);
-            return;
+            if p'' <= 0.5 {
+              p'' := 2.0 * (p'' as real);
+              assert ProbBernoulliCurried(p', s') == ProbBernoulliCurried(p'', s);
+              assert ProbBernoulliCurried(p, old(s)) == ProbBernoulliCurried(p', s');
+              assert ProbBernoulliCurried(p, old(s)) == ProbBernoulliCurried(p'', s);
+              assert !end && ProbBernoulliCurried(p, old(s)) == ProbBernoulliCurried(p'', s);
+              assert (!end && ProbBernoulliCurried(p, old(s)) == ProbBernoulliCurried(p'', s)) || (end && ProbBernoulliCurried(p, old(s)) == (c, s));
+            } else {
+              c := true;
+              end := true;
+              assert ProbBernoulliCurried(p', s') == (c, s);
+              assert ProbBernoulliCurried(p, old(s)) == ProbBernoulliCurried(p', s');
+              assert end && ProbBernoulliCurried(p, old(s)) == (c, s);
+              assert (!end && ProbBernoulliCurried(p, old(s)) == ProbBernoulliCurried(p'', s)) || (end && ProbBernoulliCurried(p, old(s)) == (c, s));
+            }
           }
         }
       }
+
+      assert (end && ProbBernoulliCurried(p, old(s)) == (c, s));
+
     }
   }
 }
